Added implementation interface for invariant assignment to refinement

Normalized_Zone_Semantics_Impl_Refine.thy
@@ -25,7 +25,44 @@ begin
   apply (simp add: aux2)
   done
 
-  context Reachability_Problem
+  subsection \<open>Mapping Transitions and Invariants\<close>
+
+  type_synonym
+    ('a, 'c, 'time, 's) transition_fun = "'s \<Rightarrow> (('c, 'time) cconstraint * 'a * 'c list * 's) list"
+  
+  definition transition_\<alpha> :: "('a, 'c, 'time, 's) transition_fun \<Rightarrow> ('a, 'c, 'time, 's) transition set"
+  where
+    "transition_\<alpha> f = {(s, t) | s t. t \<in> set (f s)}"
+
+  definition transition_rel where
+    "transition_rel = (br transition_\<alpha> (\<lambda>_. True))"
+
+  (*
+  definition inv_\<alpha> :: "('c, 'time, 's) invassn \<Rightarrow> _"
+  where
+    "inv_\<alpha> f = {(s, t) | s t. t \<in> set (f s)}"
+  
+  term inv_\<alpha>
+  
+  *)
+
+  term b_rel  
+
+  definition inv_rel where -- "Invariant assignments for a restricted state set"
+    (* XXX Or use "inv_rel X = Id_on X \<rightarrow> Id" ? *)
+    "inv_rel X = b_rel (\<lambda> x. x \<in> X) \<rightarrow> Id"
+
+  (* XXX Map from automaton? *)
+  definition state_set :: "('a, 'c, 'time, 's) transition set \<Rightarrow> 's set" where
+    "state_set T = fst ` T \<union> (snd o snd o snd o snd) ` T"
+
+  locale Reachability_Problem_Impl = Reachability_Problem A for A :: "('a, nat, int, 's) ta" +
+    fixes trans_fun :: "('a, nat, int, 's) transition_fun"
+      and inv_fun :: "(nat, int, 's) invassn"
+    assumes trans_fun: "(trans_fun, trans_of A) \<in> transition_rel"
+        and inv_fun: "(inv_fun, inv_of A) \<in> inv_rel (state_set (trans_of A))"
+        (* XXX *)
+        and start_location_in_states: "l\<^sub>0 \<in> state_set (trans_of A)"
   begin
 
   thm step_impl.intros
@@ -129,11 +166,26 @@ begin
 
   lemma [def_pat_rules]: "dbm_subset $ (Reachability_Problem.n $ A) \<equiv> PR_CONST (dbm_subset n)" by simp
 
+  abbreviation "location_rel \<equiv> b_rel (\<lambda> x. x \<in> state_set (trans_of A))"
+
+  abbreviation "location_assn \<equiv> pure location_rel"
+
   abbreviation "state_assn \<equiv> prod_assn id_assn (mtx_assn n)"
 
+  abbreviation "state_assn' \<equiv> prod_assn location_assn (mtx_assn n)"
+
+  context
+  begin
+
+  lemma [sepref_import_param]:
+    "(op =, op =) \<in> location_rel \<rightarrow> location_rel \<rightarrow> Id"
+  by auto
+
   sepref_definition subsumes_impl is
-    "uncurry (RETURN oo subsumes)" :: "state_assn\<^sup>k *\<^sub>a state_assn\<^sup>k \<rightarrow>\<^sub>a bool_assn"
-  unfolding subsumes_def by sepref
+    "uncurry (RETURN oo subsumes)" :: "state_assn'\<^sup>k *\<^sub>a state_assn'\<^sup>k \<rightarrow>\<^sub>a bool_assn"
+  unfolding subsumes_def short_circuit_conv by sepref
+
+  end
 
   (* XXX Somewhat peculiar use of the zero instance for DBM entries *)
   lemma init_dbm_alt_def:
@@ -154,10 +206,12 @@ begin
 
   sepref_register l\<^sub>0
 
-  lemma [sepref_import_param]: "(l\<^sub>0, l\<^sub>0) \<in> Id" by simp
+  lemma [sepref_import_param]:
+    "(l\<^sub>0, l\<^sub>0) \<in> location_rel"
+  using start_location_in_states by auto
 
   sepref_definition a\<^sub>0_impl is
-    "uncurry0 (RETURN a\<^sub>0)" :: "unit_assn\<^sup>k \<rightarrow>\<^sub>a state_assn"
+    "uncurry0 (RETURN a\<^sub>0)" :: "unit_assn\<^sup>k \<rightarrow>\<^sub>a state_assn'"
   unfolding a\<^sub>0_def by sepref
 
   term F term F_rel
@@ -176,12 +230,12 @@ begin
   lemma [sepref_import_param]: "(F, F) \<in> Id" by simp
 
   (* XXX Better implementation? *)
-  lemma [sepref_import_param]: "(List.member, List.member) \<in> Id \<rightarrow> Id \<rightarrow> Id" by simp
+  lemma [sepref_import_param]: "(List.member, List.member) \<in> Id \<rightarrow> location_rel \<rightarrow> Id" by auto
 
   term check_diag_impl
 
   sepref_definition F_impl is
-    "RETURN o F_rel" :: "state_assn\<^sup>k \<rightarrow>\<^sub>a bool_assn"
+    "RETURN o F_rel" :: "state_assn'\<^sup>k \<rightarrow>\<^sub>a bool_assn"
   unfolding F_rel_alt_def by sepref
 
   definition "inv_of_A = inv_of A"
@@ -202,11 +256,11 @@ begin
 
   sepref_register reset_canonical_upd
 
-  sepref_register "PR_CONST (Reachability_Problem.inv_of_A A)"
+  sepref_register "PR_CONST (Reachability_Problem_Impl.inv_of_A A)"
 
   end
 
-  definition "inv_map_assn B = pure (Id \<rightarrow> the_pure B)"
+  (* definition "inv_map_assn B = pure (Id \<rightarrow> the_pure B)" *)
 
   lemma trans_fun_clock_bounds3:
     "\<forall> c \<in> collect_clks (inv_of A l). c \<le> n"
@@ -228,22 +282,52 @@ begin
     with trans_fun_clock_bounds3 show ?thesis by auto
   qed
 
+  lemma inv_fun_rel:
+    assumes "l \<in> state_set (trans_of A)"
+    shows "(inv_fun l, inv_of A l) \<in> \<langle>\<langle>nbn_rel (Suc n), int_rel\<rangle>acconstraint_rel\<rangle>list_rel"
+  proof -
+    have "(xs, xs) \<in> \<langle>\<langle>nbn_rel (Suc n), int_rel\<rangle>acconstraint_rel\<rangle>list_rel"
+      if "\<forall> c \<in> collect_clks xs. c \<le> n" for xs
+    using that
+      apply (induction xs)
+      apply simp
+      apply simp
+      subgoal for a
+        apply (cases a)
+      by (auto simp: acconstraint_rel_def p2rel_def rel2p_def)
+    done
+    moreover have
+      "inv_fun l = inv_of A l"
+    using inv_fun assms unfolding inv_rel_def b_rel_def fun_rel_def by auto
+    ultimately show ?thesis using trans_fun_clock_bounds3 by auto
+  qed
+
  (*
  lemma [sepref_fr_rules]:
   "inv_map_assn (list_assn (acconstraint_assn (clock_assn n) int_assn)) inv_of_A inv_of_A"
 *)
 
- lemma [sepref_fr_rules]:
+ lemma (* [sepref_fr_rules]: *)
     shows "(return o inv_of_A, RETURN o PR_CONST inv_of_A) \<in> id_assn\<^sup>k \<rightarrow>\<^sub>a list_assn (acconstraint_assn (clock_assn n) int_assn)"
   using assms inv_of_rel
-  apply (simp add: aconstraint_assn_pure_conv list_assn_pure_conv inv_map_assn_def inv_of_A_def)
+  apply (simp add: aconstraint_assn_pure_conv list_assn_pure_conv inv_of_A_def)
   apply sepref_to_hoare
-  apply (sep_auto simp: inv_map_assn_def pure_def)
+  apply (sep_auto simp: pure_def)
+  done
+
+  lemma [sepref_fr_rules]:
+    shows
+    "(return o inv_fun, RETURN o PR_CONST inv_of_A)
+    \<in> location_assn\<^sup>k \<rightarrow>\<^sub>a list_assn (acconstraint_assn (clock_assn n) int_assn)"
+  using assms inv_fun_rel
+  apply (simp add: aconstraint_assn_pure_conv list_assn_pure_conv inv_of_A_def)
+  apply sepref_to_hoare
+  apply (sep_auto simp: pure_def)
   done
  
 
   term pure
-
+(*
   lemma [sepref_fr_rules]:
     assumes "CONSTRAINT (IS_PURE IS_BELOW_ID) B"
     shows "(return o inv_of, RETURN o inv_of) \<in> id_assn\<^sup>k \<rightarrow>\<^sub>a inv_map_assn (list_assn (acconstraint_assn (clock_assn n) int_assn))"
@@ -251,10 +335,12 @@ begin
   apply sepref_to_hoare
   apply (sep_auto simp: IS_BELOW_ID_def IS_PURE_def inv_map_assn_def pure_def split: prod.split)
 oops
+*)
 (*  using assms by sepref_to_hoare (sep_auto simp: IS_BELOW_ID_def IS_PURE_def inv_map_assn_def pure_def) *)
 
-  definition inv_map_lookup :: "('c \<Rightarrow> 'b) \<Rightarrow> _" where "inv_map_lookup M a = M a"
+  (* definition inv_map_lookup :: "('c \<Rightarrow> 'b) \<Rightarrow> _" where "inv_map_lookup M a = M a" *)
 
+(*
   lemma inv_map_lookup_fr_rule[sepref_fr_rules]:
     assumes "CONSTRAINT (IS_PURE IS_ID) B"
     shows
@@ -263,6 +349,7 @@ oops
   using assms by sepref_to_hoare (sep_auto simp: IS_ID_def IS_PURE_def inv_map_assn_def pure_def)
 
   thm inv_map_lookup_fr_rule[to_hnr]
+*)
 
   term inv_of
 
@@ -270,7 +357,7 @@ oops
 
   thm sepref_frame_normrel_eqs
 
-  sepref_register inv_map_lookup
+  (* sepref_register inv_map_lookup *)
 
   term fw_impl term fw_impl'
 
@@ -333,10 +420,25 @@ oops
     "(g, a, r, l') \<in> set (trans_fun l) \<Longrightarrow> \<forall> c \<in> collect_clks g. c \<le> n"
   using n_bounded collect_clocks_clk_set[OF trans_fun_trans_of] unfolding X_def by fastforce
 
+  lemma trans_fun_states1:
+    "(g, a, r, l') \<in> set (trans_fun l) \<Longrightarrow> l \<in> state_set (trans_of A)"
+  unfolding state_set_def
+   apply (drule trans_fun_trans_of)
+   apply (rule UnI1)
+  by force
+
+  lemma trans_fun_states2:
+    "(g, a, r, l') \<in> set (trans_fun l) \<Longrightarrow> l' \<in> state_set (trans_of A)"
+  unfolding state_set_def
+   apply (drule trans_fun_trans_of)
+   apply (rule UnI2)
+  by force
+
   abbreviation "clock_rel \<equiv> nbn_rel (Suc n)"
 
-  lemma [sepref_import_param]:
-    "(trans_fun, trans_fun) \<in> Id \<rightarrow> \<langle>\<langle>\<langle>clock_rel, int_rel\<rangle> acconstraint_rel\<rangle> list_rel \<times>\<^sub>r Id \<times>\<^sub>r \<langle>clock_rel\<rangle> list_rel \<times>\<^sub>r Id\<rangle> list_rel"
+  lemma (* [sepref_import_param]: *)
+    "(trans_fun, trans_fun)
+    \<in> Id \<rightarrow> \<langle>\<langle>\<langle>clock_rel, int_rel\<rangle> acconstraint_rel\<rangle> list_rel \<times>\<^sub>r Id \<times>\<^sub>r \<langle>clock_rel\<rangle> list_rel \<times>\<^sub>r Id\<rangle> list_rel"
   apply (rule fun_relI)
   apply simp
   subgoal for x x'
@@ -371,10 +473,92 @@ oops
   qed
   done
 
+  lemma (* [sepref_import_param]: *)
+    "(trans_fun, trans_fun)
+    \<in> Id \<rightarrow> \<langle>\<langle>\<langle>clock_rel, int_rel\<rangle> acconstraint_rel\<rangle> list_rel \<times>\<^sub>r Id \<times>\<^sub>r \<langle>clock_rel\<rangle> list_rel \<times>\<^sub>r location_rel\<rangle> list_rel"
+  apply (rule fun_relI)
+  apply simp
+  subgoal for x x'
+  proof -
+    { fix l :: "((nat, int) acconstraint list \<times> 'a \<times> nat list \<times> 's) list"
+      assume "\<forall> g a r l'. (g, a, r, l') \<in> set l \<longrightarrow> (\<forall> c \<in> collect_clks g. c \<le> n) \<and> (\<forall> c \<in> set r. c \<le> n) \<and> l' \<in> state_set (trans_of A)"
+      then have "(l, l) \<in> \<langle>\<langle>\<langle>nbn_rel (Suc n), int_rel\<rangle>acconstraint_rel\<rangle>list_rel \<times>\<^sub>r Id \<times>\<^sub>r \<langle>nbn_rel (Suc n)\<rangle>list_rel \<times>\<^sub>r location_rel\<rangle>list_rel"
+      proof (induction l)
+        case Nil then show ?case by simp
+      next
+        case (Cons x xs)
+        then obtain g a r l' where [simp]: "x = (g, a, r, l')" by (cases x)
+        from Cons.prems have r_bounds: "\<forall> c \<in> set r. c \<le> n" by auto
+        from Cons.prems have "\<forall> c \<in> collect_clks g. c \<le> n" by auto
+        then have "(g, g) \<in> \<langle>\<langle>nbn_rel (Suc n), int_rel\<rangle>acconstraint_rel\<rangle>list_rel"
+          apply (induction g)
+          apply simp
+          apply simp
+          subgoal for a
+          apply (cases a)
+          by (auto simp: acconstraint_rel_def p2rel_def rel2p_def)
+        done
+        moreover from r_bounds have "(r, r) \<in> \<langle>nbn_rel (Suc n)\<rangle>list_rel" by (induction r) auto
+        moreover from Cons.prems have "(l', l') \<in> location_rel" by auto
+        ultimately have
+          "(x, x) \<in> \<langle>\<langle>nbn_rel (Suc n), int_rel\<rangle>acconstraint_rel\<rangle>list_rel \<times>\<^sub>r Id \<times>\<^sub>r \<langle>nbn_rel (Suc n)\<rangle>list_rel \<times>\<^sub>r location_rel"
+        by simp
+        moreover from Cons have
+          "(xs, xs) \<in> \<langle>\<langle>\<langle>nbn_rel (Suc n), int_rel\<rangle>acconstraint_rel\<rangle>list_rel \<times>\<^sub>r Id \<times>\<^sub>r \<langle>nbn_rel (Suc n)\<rangle>list_rel \<times>\<^sub>r location_rel\<rangle>list_rel"
+        by force
+        ultimately show ?case by simp
+      qed
+    }
+    from this[of "trans_fun x'"] trans_fun_clock_bounds1 trans_fun_clock_bounds2 trans_fun_states2 show ?thesis by auto
+  qed
+  done
+
+  lemma [sepref_import_param]:
+    "(trans_fun, trans_fun)
+    \<in> location_rel \<rightarrow> \<langle>\<langle>\<langle>clock_rel, int_rel\<rangle> acconstraint_rel\<rangle> list_rel \<times>\<^sub>r Id \<times>\<^sub>r \<langle>clock_rel\<rangle> list_rel \<times>\<^sub>r location_rel\<rangle> list_rel"
+  apply (rule fun_relI)
+  apply simp
+  subgoal for x x'
+  proof -
+    { fix l :: "((nat, int) acconstraint list \<times> 'a \<times> nat list \<times> 's) list"
+      assume "\<forall> g a r l'. (g, a, r, l') \<in> set l \<longrightarrow> (\<forall> c \<in> collect_clks g. c \<le> n) \<and> (\<forall> c \<in> set r. c \<le> n) \<and> l' \<in> state_set (trans_of A)"
+      then have "(l, l) \<in> \<langle>\<langle>\<langle>nbn_rel (Suc n), int_rel\<rangle>acconstraint_rel\<rangle>list_rel \<times>\<^sub>r Id \<times>\<^sub>r \<langle>nbn_rel (Suc n)\<rangle>list_rel \<times>\<^sub>r location_rel\<rangle>list_rel"
+      proof (induction l)
+        case Nil then show ?case by simp
+      next
+        case (Cons x xs)
+        then obtain g a r l' where [simp]: "x = (g, a, r, l')" by (cases x)
+        from Cons.prems have r_bounds: "\<forall> c \<in> set r. c \<le> n" by auto
+        from Cons.prems have "\<forall> c \<in> collect_clks g. c \<le> n" by auto
+        then have "(g, g) \<in> \<langle>\<langle>nbn_rel (Suc n), int_rel\<rangle>acconstraint_rel\<rangle>list_rel"
+          apply (induction g)
+          apply simp
+          apply simp
+          subgoal for a
+          apply (cases a)
+          by (auto simp: acconstraint_rel_def p2rel_def rel2p_def)
+        done
+        moreover from r_bounds have "(r, r) \<in> \<langle>nbn_rel (Suc n)\<rangle>list_rel" by (induction r) auto
+        moreover from Cons.prems have "(l', l') \<in> location_rel" by auto
+        ultimately have
+          "(x, x) \<in> \<langle>\<langle>nbn_rel (Suc n), int_rel\<rangle>acconstraint_rel\<rangle>list_rel \<times>\<^sub>r Id \<times>\<^sub>r \<langle>nbn_rel (Suc n)\<rangle>list_rel \<times>\<^sub>r location_rel"
+        by simp
+        moreover from Cons have
+          "(xs, xs) \<in> \<langle>\<langle>\<langle>nbn_rel (Suc n), int_rel\<rangle>acconstraint_rel\<rangle>list_rel \<times>\<^sub>r Id \<times>\<^sub>r \<langle>nbn_rel (Suc n)\<rangle>list_rel \<times>\<^sub>r location_rel\<rangle>list_rel"
+        by force
+        ultimately show ?case by simp
+      qed
+    }
+    from this[of "trans_fun x'"] trans_fun_clock_bounds1 trans_fun_clock_bounds2 trans_fun_states2 show ?thesis by auto
+  qed
+  done
+
+  (*
   lemma [sepref_fr_rules]:
     "(return o trans_fun, RETURN o trans_fun) \<in> id_assn\<^sup>k \<rightarrow>\<^sub>a list_assn (prod_assn (list_assn (acconstraint_assn (clock_assn n) int_assn)) (prod_assn id_assn (prod_assn id_assn id_assn)))"
   apply (simp add: list_assn_pure_conv)
   oops
+  *)
 
   lemmas [sepref_fr_rules] =
     abstr_upd_impl.refine up_canonical_upd_impl.refine norm_upd_impl.refine
@@ -386,6 +570,7 @@ oops
     "hn_val (b_rel P) a b \<Longrightarrow>\<^sub>t hn_val Id a b"
   by (rule enttI) (sep_auto simp: hn_ctxt_def pure_def)
 
+
   sepref_register op_HOL_list_empty
 
   term "a \<or>\<^sub>A b"
@@ -395,16 +580,15 @@ oops
     "hn_val Id a b \<or>\<^sub>A hn_val (b_rel p) a b \<Longrightarrow>\<^sub>t hn_val Id a b"
   by (simp add: b_rel_subtype entt_disjE)+
 
-
-  lemma [def_pat_rules]: "(Reachability_Problem.inv_of_A $ A) \<equiv> PR_CONST inv_of_A" by simp
+  lemma [def_pat_rules]: "(Reachability_Problem_Impl.inv_of_A $ A) \<equiv> PR_CONST inv_of_A" by simp
 
   lemmas [safe_constraint_rules] = CN_FALSEI[of is_pure "asmtx_assn n a" for n a]
 
   lemma [sepref_opt_simps]: "UNPROTECT n = n" by simp
 
   sepref_definition succs_impl is
-    "RETURN o succs" :: "state_assn\<^sup>k \<rightarrow>\<^sub>a list_assn state_assn"
-  unfolding comp_def succs'_succs[symmetric] succs'_def inv_map_lookup_def[symmetric, of "inv_of A"]
+    "RETURN o succs" :: "state_assn'\<^sup>k \<rightarrow>\<^sub>a list_assn state_assn'"
+  unfolding comp_def succs'_succs[symmetric] succs'_def (* inv_map_lookup_def[symmetric, of "inv_of A"] *)
   FW''_def[symmetric] rev_map_fold reset'_upd_def inv_of_A_def[symmetric]
   apply (rewrite "HOL_list.fold_custom_empty")
 using [[goals_limit = 1]]
@@ -420,7 +604,7 @@ done
    apply (auto; fail)
   by (safe, erule step_impl.cases; force)
 
-  sublocale Worklist2 E a\<^sub>0 F_rel subsumes succs state_assn succs_impl a\<^sub>0_impl F_impl subsumes_impl
+  sublocale Worklist2 E a\<^sub>0 F_rel subsumes succs state_assn' succs_impl a\<^sub>0_impl F_impl subsumes_impl
   by standard (rule a\<^sub>0_impl.refine F_impl.refine subsumes_impl.refine succs_impl.refine)+
 
 (*
